é¢˜ç›®ç­‰ä»·äºç ”ç©¶æé™å®šä¹‰çš„å‡½æ•°
$$
f(x)=\lim_{n\to\infty}\frac{1+x}{1+n x^{2n}}
$$
å¹¶åˆ¤æ–­å®ƒåœ¨ (x=1) ä¸ (x=-1) å¤„çš„è¿ç»­æ€§ã€‚


---

## ç¬¬ä¸€æ­¥ï¼šå…ˆæ±‚å‡½æ•°çš„è§£æè¡¨è¾¾å¼ï¼ˆåˆ†æƒ…å½¢ï¼‰

å…³é”®åœ¨äº $x^{2n}$ éš $n\to\infty$ çš„æé™è¡Œä¸ºã€‚

### æƒ…å½¢ 1ï¼š(|x|<1)

$$
x^{2n}\to 0 \quad\Rightarrow\quad n x^{2n}\to 0
$$

å› æ­¤
$$
f(x)=\frac{1+x}{1+0}=1+x
$$

---

### æƒ…å½¢ 2ï¼š(|x|>1)

$$
x^{2n}\to +\infty \quad\Rightarrow\quad n x^{2n}\to +\infty
$$

å› æ­¤
$$
f(x)=\frac{1+x}{+\infty}=0
$$

---

### æƒ…å½¢ 3ï¼š(|x|=1)

#### (1) (x=1)

$$
f(1)=\lim_{n\to\infty}\frac{2}{1+n} = 0
$$

#### (2) (x=-1)

$$
f(-1)=\lim_{n\to\infty}\frac{0}{1+n}=0
$$

---

## ç¬¬äºŒæ­¥ï¼šå†™å‡ºåˆ†æ®µå‡½æ•°

$$
f(x)=
\begin{cases}
1+x, & |x|<1 \\
0, & |x|\ge 1
\end{cases}
$$

---

## ç¬¬ä¸‰æ­¥ï¼šåˆ¤æ–­è¿ç»­æ€§

### åœ¨ (x=1)

* å·¦æé™ï¼š
  $$
  \lim_{x\to1^-} f(x)=1+1=2
  $$
* å‡½æ•°å€¼ï¼š
  $$
  f(1)=0
  $$

âŒ å·¦æé™ $\ne$ å‡½æ•°å€¼ â†’ **ä¸è¿ç»­**

---

### åœ¨ (x=-1)

* å³æé™ï¼š
  $$
  \lim_{x\to(-1)^+} f(x)=1+(-1)=0
  $$
* å·¦æé™ï¼š
  $$
  \lim_{x\to(-1)^-} f(x)=0
  $$
* å‡½æ•°å€¼ï¼š
  $$
  f(-1)=0
  $$

âœ… æé™ = å‡½æ•°å€¼ â†’ **è¿ç»­**

---

## âœ… æœ€ç»ˆç­”æ¡ˆ

**(D) åœ¨ (x=1) å¤„ä¸è¿ç»­ï¼Œåœ¨ (x=-1) å¤„è¿ç»­**


---
$$
I=\int_a^{a+k\pi}|\sin x|,dx,\quad k\in\mathbb Z
$$

æ³¨æ„åˆ° $|\sin x|$ çš„å‘¨æœŸæ˜¯ $\pi$ï¼Œå› ä¸º
$$
|\sin(x+\pi)|=|-\sin x|=|\sin x|.
$$
å› æ­¤ä»»æ„é•¿åº¦ä¸º $\pi$ çš„åŒºé—´ä¸Šç§¯åˆ†éƒ½ç›¸åŒï¼š
$$
\int_t^{t+\pi}|\sin x|,dx=\int_0^\pi \sin x,dx=2.
$$

æŠŠåŒºé—´ $[a,\ a+k\pi]$ åˆ†æˆ $k$ ä¸ªé•¿åº¦ä¸º $\pi$ çš„å°æ®µï¼ˆ$k>0$ æ—¶ï¼‰ï¼š
$$
I=\sum_{j=0}^{k-1}\int_{a+j\pi}^{a+(j+1)\pi}|\sin x|,dx
= \sum_{j=0}^{k-1}2 = 2k.
$$
è‹¥ $k<0$ï¼Œåˆ™ç§¯åˆ†ä¸Šä¸‹é™å¯¹è°ƒä¼šå¸¦æ¥ç¬¦å·ï¼Œç»“è®ºä»ä¸º $I=2k$ï¼ˆ$k=0$ æ—¶ $I=0$ï¼‰ã€‚

æ‰€ä»¥ (I) **åªä¸ (k) æœ‰å…³ï¼Œä¸ (a) æ— å…³**ã€‚

**ç­”æ¡ˆï¼š (B) åªä¸ (k) æœ‰å…³ã€‚**

---
No problem â€” letâ€™s go **very slowly and intuitively**, step by step ğŸ˜Š

---

## Step 1ï¼šå…ˆçœ‹å‡½æ•°é•¿ä»€ä¹ˆæ ·

æˆ‘ä»¬ç ”ç©¶çš„æ˜¯
$$
|\sin x|
$$

å…³é”®äº‹å®åªæœ‰ä¸€ä¸ªï¼š

> **$|\sin x|$ çš„å›¾åƒæ¯éš” $\pi$ å°±å®Œå…¨é‡å¤ä¸€æ¬¡**

ä¹Ÿå°±æ˜¯è¯´ï¼š
$$
|\sin(x+\pi)|=|\sin x|
$$

æ‰€ä»¥å®ƒçš„**å‘¨æœŸæ˜¯ $\pi$**ã€‚

---

## Step 2ï¼šä¸€ä¸ªæœ€é‡è¦çš„å›ºå®šç»“æœï¼ˆæ ¸å¿ƒï¼‰

ä¸ç®¡ä»å“ªé‡Œå¼€å§‹ï¼Œåªè¦åŒºé—´é•¿åº¦æ˜¯ $\pi$ï¼Œç§¯åˆ†å€¼éƒ½ä¸€æ ·ï¼š

$$
\int_{t}^{t+\pi}|\sin x|,dx = 2 \quad (\text{å¯¹ä»»æ„ } t)
$$

ä¸ºä»€ä¹ˆï¼Ÿ
å› ä¸ºåœ¨ $[0,\pi]$ ä¸Šï¼š
$$
|\sin x|=\sin x
$$
$$
\int_0^\pi \sin x,dx = 2
$$

è€Œå‘¨æœŸæ€§ä¿è¯äº† **æ¯ä¸€ä¸ªé•¿åº¦ä¸º $\pi$ çš„åŒºé—´â€œé¢ç§¯â€éƒ½ç­‰äº 2**ã€‚

ğŸ‘‰ è®°ä½è¿™å¥è¯å°±å¤Ÿäº†ã€‚

---

## Step 3ï¼šå†çœ‹ä½ çš„ç§¯åˆ†åŒºé—´

$$
I=\int_a^{a+k\pi}|\sin x|,dx
$$

* èµ·ç‚¹æ˜¯ **$a$**
* ç»ˆç‚¹æ˜¯ **$a+k\pi$**
* åŒºé—´é•¿åº¦æ˜¯ï¼š
  $$
  (a+k\pi)-a = k\pi
  $$

âš ï¸ **æ³¨æ„**ï¼šä¸ç®¡ $a$ æ˜¯å¤šå°‘ï¼ŒåŒºé—´é•¿åº¦æ°¸è¿œæ˜¯ $k\pi$ã€‚

---

## Step 4ï¼šæŠŠåŒºé—´â€œåˆ‡å—â€

é•¿åº¦æ˜¯ $k\pi$ï¼Œè€Œ **æ¯ $\pi$ çš„é¢ç§¯æ˜¯ 2**ï¼š

* ç¬¬ 1 ä¸ª $\pi$ï¼šé¢ç§¯ 2
* ç¬¬ 2 ä¸ª $\pi$ï¼šé¢ç§¯ 2
* â€¦â€¦
* ä¸€å…± **$k$ ä¸ª $\pi$**

æ‰€ä»¥ï¼š
$$
I = 2 + 2 + \cdots + 2 = 2k
$$

---

## Step 5ï¼šå…³é”®ç»“è®ºï¼ˆæœ€é‡è¦ï¼‰

$$
I = 2k
$$

* **æ²¡æœ‰ $a$**
* **åªæœ‰ $k$**

ä¹Ÿå°±æ˜¯è¯´ï¼š

> æ”¹å˜èµ·ç‚¹ $a$ï¼Œåªæ˜¯æŠŠåŒºé—´åœ¨å›¾åƒä¸Šâ€œå·¦å³å¹³ç§»â€ï¼Œ
> **ä½†é¢ç§¯ä¸å˜**ã€‚

---

## æœ€ç»ˆç­”æ¡ˆ

$$
\boxed{\text{(B) åªä¸ } k \text{ æœ‰å…³}}
$$

---

### ä¸€å¥è¯è®°å¿†æ³• ğŸ’¡

> **å‘¨æœŸå‡½æ•° + ç§¯åˆ†åŒºé—´é•¿åº¦æ˜¯æ•´æ•°ä¸ªå‘¨æœŸ â‡’ ä¸èµ·ç‚¹æ— å…³**

---
Great question â€” this is the **key confusion point**, so letâ€™s focus **only** on this and explain **why** it is true, very concretely.

---

## Why is

$$
|\sin x| = \sin x \quad \text{on } [0,\pi]?
$$

### Step 1: Think about the sine graph

On the interval
$$
0 \le x \le \pi
$$

the sine curve:

* starts at $0$ when (x=0)
* rises to $1$ at $x=\tfrac{\pi}{2}$
* goes back to $0$ at $x=\pi$

ğŸ‘‰ **It is never negative on this interval.**

So for every $x\in[0,\pi]$:
$$
\sin x \ge 0
$$

---

## Step 2: What does absolute value do?

By definition:
$$
|y| =
\begin{cases}
y, & y\ge 0 \\
-y, & y<0
\end{cases}
$$

Since $\sin x \ge 0$ on $[0,\pi]$,
$$
|\sin x| = \sin x \quad \text{on } [0,\pi]
$$

Thatâ€™s all â€” **nothing more complicated than that**.

---

## Step 3: Now the integral becomes simple

Because the absolute value does nothing on this interval:
$$
\int_0^\pi |\sin x|,dx = \int_0^\pi \sin x,dx
$$

We already know:
$$
\int \sin x,dx = -\cos x
$$

So:
$$
\int_0^\pi \sin x,dx
= [-\cos x]_0^\pi
= (-\cos\pi)-(-\cos0)
= (1)-(-1)
= 2
$$

---

## Step 4: Why this matters

This tells us:

> **Every â€œhumpâ€ of $|\sin x|$ over length $\pi$ has area 2.**

Thatâ€™s why:
$$
\int_t^{t+\pi}|\sin x|,dx = 2 \quad \text{(no matter where you start)}
$$

---

## One-sentence intuition ğŸŒ±

> On $[0,\pi]$, sine is already positive, so the absolute value does nothing â€” it just keeps the same curve.

---

If you want, I can also explain:

* **why the area is the same starting anywhere**, or
* **what changes on $[\pi,2\pi]$**

Just tell me ğŸ‘

---

å¾ˆå¥½ï¼Œè¿™ä¸ªé—®é¢˜é—®å¾—**éå¸¸å…³é”®**ã€‚æˆ‘ä»¬å°±åªè§£é‡Šè¿™ä¸€ç‚¹ï¼š

> **ä¸ºä»€ä¹ˆå½“ (k<0) æ—¶ï¼Œä¼šè¯´â€œç§¯åˆ†ä¸Šä¸‹é™å¯¹è°ƒâ€ï¼Ÿ**

---

## ä¸€ã€å…ˆçœ‹ä½ çš„ç§¯åˆ†æœ¬èº«

$$
I=\int_a^{a+k\pi}|\sin x|,dx
$$

å¦‚æœ

* $k>0$ï¼š
  $$
  a+k\pi > a \quad(\text{ä¸‹é™å°ï¼Œä¸Šé™å¤§ï¼Œæ­£å¸¸})
  $$

* **$k<0$ï¼š**
  $$
  a+k\pi < a
  $$

è¿™æ—¶å‘ç”Ÿäº†ä»€ä¹ˆï¼Ÿ

ğŸ‘‰ **ç§¯åˆ†çš„â€œä¸‹é™æ¯”ä¸Šé™å¤§â€äº†**ã€‚

---

## äºŒã€å®šç§¯åˆ†çš„ä¸€ä¸ªåŸºæœ¬è§„åˆ™ï¼ˆå¿…é¡»è®°ä½ï¼‰

å¯¹ä»»ä½•å‡½æ•° $f(x)$ï¼Œéƒ½æœ‰ï¼š

$$
\boxed{\int_b^a f(x),dx = -\int_a^b f(x),dx}
$$

è¿™å°±å«åšï¼š

> **ç§¯åˆ†ä¸Šä¸‹é™å¯¹è°ƒï¼Œç§¯åˆ†å€¼å˜å·**

è¿™æ˜¯å®šç§¯åˆ†çš„å®šä¹‰æ€§è´¨ï¼Œä¸æ˜¯æŠ€å·§ã€‚

---

## ä¸‰ã€æŠŠå®ƒç”¨åˆ°è¿™é‡Œï¼ˆä¸€æ­¥ä¸€æ­¥ï¼‰

å½“ $k<0$ æ—¶ï¼š

$$
I=\int_a^{a+k\pi}|\sin x|,dx
$$

å› ä¸º $a+k\pi<a$ï¼Œæˆ‘ä»¬æŠŠä¸Šä¸‹é™å¯¹è°ƒï¼š

$$
I = -\int_{a+k\pi}^{a}|\sin x|,dx
$$

ç°åœ¨æ³¨æ„ï¼š

$$
a-(a+k\pi) = -k\pi
$$

ğŸ‘‰ åŒºé—´é•¿åº¦æ˜¯ **$|k|\pi$**
ğŸ‘‰ ä¸€å…±æœ‰ **$|k|$** ä¸ªé•¿åº¦ä¸º $\pi$ çš„å‘¨æœŸ

è€Œæ¯ä¸ªå‘¨æœŸçš„é¢ç§¯ä»ç„¶æ˜¯ 2ï¼Œæ‰€ä»¥ï¼š

$$
\int_{a+k\pi}^{a}|\sin x|,dx = 2|k|
$$

äºæ˜¯ï¼š

$$
I = -2|k|
$$

ä½†å½“ $k<0$ æ—¶ï¼Œ$|k|=-k$ï¼Œæ‰€ä»¥ï¼š

$$
I = -2(-k)=2k
$$

---

## å››ã€ä¸ºä»€ä¹ˆä¸€å®šè¦è¿™æ ·è§„å®šï¼Ÿï¼ˆç›´è§‰è§£é‡Šï¼‰

ä½ å¯ä»¥æŠŠå®šç§¯åˆ†ç†è§£æˆï¼š

> **â€œä»å·¦èµ°åˆ°å³ï¼Œæ›²çº¿æ‰«è¿‡çš„å¸¦ç¬¦å·é¢ç§¯â€**

* ä»å°åˆ°å¤§ï¼ˆæ­£å¸¸æ–¹å‘ï¼‰ï¼šæ­£å·
* ä»å¤§åˆ°å°ï¼ˆåæ–¹å‘ï¼‰ï¼šè´Ÿå·

å°±åƒèµ°è·¯ï¼š

* å‘å‰èµ°ï¼š+
* å‘åèµ°ï¼šâˆ’

æ‰€ä»¥å½“ä¸Šä¸‹é™åäº†ï¼Œæ–¹å‘åäº†ï¼Œç¬¦å·å°±å¿…é¡»åã€‚

---

## äº”ã€æ€»ç»“ä¸€å¥è¯ï¼ˆè€ƒè¯•ç”¨ï¼‰

> å½“ $k<0$ æ—¶ï¼Œç§¯åˆ†åŒºé—´æ–¹å‘åäº†ï¼Œ
> åˆ©ç”¨å®šç§¯åˆ†æ€§è´¨
> $\displaystyle \int_b^a f(x),dx=-\int_a^b f(x),dx$ï¼Œ
> å› æ­¤â€œä¸Šä¸‹é™å¯¹è°ƒå¹¶å˜å·â€ã€‚



---

é¢˜ç›®ç»™çš„æ˜¯

$$
\int_{x=\pi/6}^{\pi/2}!dx\int_{y=\sin x}^{1} f(x,y),dy
$$

è¿™è¡¨ç¤ºçš„ç§¯åˆ†åŒºåŸŸ (D) æ˜¯ï¼š

$$
D={(x,y)\mid \pi/6\le x\le \pi/2,\ \sin x\le y\le 1}.
$$

---

## 1ï¼‰å…ˆæŠŠåŒºåŸŸç”»åœ¨è„‘å­é‡Œï¼ˆç”¨ä¸ç­‰å¼ç†è§£ï¼‰

* $x$ åœ¨ $[\pi/6,\ \pi/2]$ ä¹‹é—´ï¼ˆç«–ç€ä¸€æ¡å¸¦çŠ¶åŒºåŸŸï¼‰
* å¯¹æ¯ä¸ªå›ºå®šçš„ $x$ï¼Œ$y$ ä» $\sin x$ åˆ° 1

ä¹Ÿå°±æ˜¯ï¼šåŒºåŸŸåœ¨æ›²çº¿ $y=\sin x$ **ä¸Šæ–¹**ï¼Œåœ¨ç›´çº¿ $y=1$ **ä¸‹æ–¹**ï¼Œå¹¶ä¸” $x$ è¢«å¤¹åœ¨ $\pi/6$ å’Œ $\pi/2$ ä¹‹é—´ã€‚

---

## 2ï¼‰æ¢é¡ºåºï¼šå…ˆç¡®å®š $y$ çš„èŒƒå›´

å½“ $x$ åœ¨ $[\pi/6,\pi/2]$ å˜åŒ–æ—¶ï¼Œ$\sin x$ çš„æœ€å°å€¼å’Œæœ€å¤§å€¼æ˜¯ï¼š

* $\sin(\pi/6)=1/2$
* $\sin(\pi/2)=1$

æ‰€ä»¥åŒºåŸŸé‡Œçš„ $y$ å–å€¼èŒƒå›´æ˜¯ï¼š

$
\boxed{\frac12 \le y \le 1}
$

---

## 3ï¼‰å›ºå®šä¸€ä¸ª $y$ï¼Œæ±‚ $x$ çš„èŒƒå›´

åŒºåŸŸæ¡ä»¶è¿˜æœ‰ï¼š$\sin x \le y$ï¼Œå¹¶ä¸” $x\in[\pi/6,\pi/2]$ã€‚

åœ¨ $[\pi/6,\pi/2]$ ä¸Šï¼Œ$\sin x$ **å•è°ƒé€’å¢**ï¼Œæ‰€ä»¥

$$
\sin x \le y \iff x \le \arcsin y
$$

å†ç»“åˆä¸‹ç•Œ $x\ge \pi/6$ï¼Œå¾—åˆ°

$$
\boxed{\pi/6 \le x \le \arcsin y}
$$

ï¼ˆæ³¨æ„ï¼šå½“ $y=1$ æ—¶ $\arcsin 1=\pi/2$ï¼Œåˆšå¥½æ¥ä¸Šã€‚ï¼‰

---

## 4ï¼‰å†™å‡ºæ¢åºåçš„ç§¯åˆ†

$$
\boxed{\int_{y=1/2}^{1}!dy\int_{x=\pi/6}^{\arcsin y} f(x,y),dx}
$$

å¯¹åº”é€‰é¡¹ **(A)**ã€‚âœ…

---

å¦‚æœä½ æ„¿æ„ï¼Œæˆ‘ä¹Ÿå¯ä»¥ç”¨ä¸€å¼ â€œåŒºåŸŸç¤ºæ„å›¾â€çš„æ–¹å¼æŠŠè¾¹ç•Œå¯¹åº”å…³ç³»å†ç›´è§‚çœ‹ä¸€éã€‚

---
Yes ğŸ‘ let me **draw it conceptually and visually explain it**.

---

## The integration region (D)

åŸç§¯åˆ†æ˜¯
$$
\int_{x=\pi/6}^{\pi/2}  dx \int_{y=\sin x}^{1} f(x,y),dy
$$

å®ƒè¡¨ç¤ºçš„åŒºåŸŸæ˜¯ï¼š

* å·¦è¾¹ç•Œï¼š$x=\pi/6$
* å³è¾¹ç•Œï¼š$x=\pi/2$
* ä¸‹è¾¹ç•Œï¼š$y=\sin x$
* ä¸Šè¾¹ç•Œï¼š$y=1$

---

## å›¾å½¢ç›´è§‚ç¤ºæ„


```
y
â†‘
1 â”€â”€â”€â”€â”€â”€â”€â”€â”€â”€â”€â”€â”€â”€â”€â”€â”€â”€â”€  y = 1
â”‚        â–ˆâ–ˆâ–ˆâ–ˆâ–ˆâ–ˆâ–ˆâ–ˆâ–ˆâ–ˆâ–ˆâ–ˆ  â† ç§¯åˆ†åŒºåŸŸ
â”‚      â–ˆâ–ˆâ–ˆâ–ˆâ–ˆâ–ˆâ–ˆâ–ˆâ–ˆâ–ˆâ–ˆâ–ˆ
â”‚    â–ˆâ–ˆâ–ˆâ–ˆâ–ˆâ–ˆâ–ˆâ–ˆâ–ˆâ–ˆâ–ˆâ–ˆ
â”‚  â–ˆâ–ˆâ–ˆâ–ˆâ–ˆâ–ˆâ–ˆâ–ˆâ–ˆâ–ˆâ–ˆâ–ˆ
â”‚â–ˆâ–ˆâ–ˆâ–ˆâ–ˆâ–ˆâ–ˆâ–ˆâ–ˆâ–ˆâ–ˆâ–ˆ
â”‚   y = sin x
â””â”€â”€â”€â”€â”€â”€â”€â”€â”€â”€â”€â”€â”€â”€â”€â”€â”€â”€â”€â”€â†’ x
   Ï€/6           Ï€/2
```

é˜´å½±éƒ¨åˆ†å°±æ˜¯ç§¯åˆ†åŒºåŸŸ (D)ã€‚

---

## ä¸ºä»€ä¹ˆæ¢åºåæ˜¯è¿™æ ·ï¼Ÿ

### â‘  çœ‹ y çš„èŒƒå›´ï¼ˆæ¨ªç€æ‰«ï¼‰

* æœ€ä½ç‚¹æ¥è‡ª $\sin(\pi/6)=1/2$
* æœ€é«˜ç‚¹æ˜¯ $1$

æ‰€ä»¥ï¼š
$$
\boxed{\frac12 \le y \le 1}
$$

---

### â‘¡ å›ºå®šä¸€ä¸ª yï¼Œçœ‹ x èƒ½å–åˆ°å“ªé‡Œ

åŒºåŸŸæ¡ä»¶æ˜¯ï¼š
$$
y \ge \sin x
$$

åœ¨ $[\pi/6,\pi/2]$ ä¸Šï¼Œ$\sin x$ **å•è°ƒé€’å¢**ï¼Œæ‰€ä»¥ï¼š

$$
\sin x \le y \iff x \le \arcsin y
$$

å†åŠ ä¸Šå·¦è¾¹ç•Œ $x\ge \pi/6$ï¼Œå¾—åˆ°ï¼š

$$
\boxed{\pi/6 \le x \le \arcsin y}
$$

---

## æœ€ç»ˆæ¢åºç»“æœï¼ˆå’Œå›¾å®Œå…¨ä¸€è‡´ï¼‰

$$
\boxed{
\int_{1/2}^{1} dy \int_{\pi/6}^{\arcsin y} f(x,y),dx
}
$$

ğŸ‘‰ **ç­”æ¡ˆï¼š (A)**

---

### ä¸€å¥è¯è®°å¿†æ³• ğŸŒ±

> **å…ˆç”»åŒºåŸŸï¼Œå†â€œæ¨ªç€æ‰«â€ï¼Œä¸‹ y ä¸Š yï¼Œå·¦ x å³ x**

å¦‚æœä½ æƒ³ï¼Œæˆ‘ä¹Ÿå¯ä»¥**ä¸€æ­¥ä¸€æ­¥æ•™ä½ æ€ä¹ˆåœ¨è€ƒè¯•ä¸­ 30 ç§’ç”»è¿™ç§å›¾**ã€‚

---
å·²çŸ¥
$$
\sum_{n=0}^\infty a_n x^n=\ln(2+x)
$$
åœ¨ $x=0$ å±•å¼€ï¼š
$$
\ln(2+x)=\ln2+\ln\left(1+\frac x2\right)
=\ln2+\sum_{m=1}^\infty (-1)^{m+1}\frac1m(\frac x2)^m \quad(|x|<2)
$$
æ‰€ä»¥å¯¹ $n\ge1$,
$$
a_n = (-1)^{n+1}\frac{1}{n2^n},\qquad a_0=\ln2.
$$

æˆ‘ä»¬è¦ç®—
$$
\sum_{n=0}^\infty na_{2n}
$$
æ³¨æ„ $n=0$ é¡¹ä¸º 0ï¼Œä» $n\ge1$ å¼€å§‹ï¼š

$$
a_{2n}=(-1)^{2n+1}\frac{1}{(2n),2^{2n}}
=-\frac{1}{2n\cdot 4^n}
$$
å› æ­¤
$$
n a_{2n}=n\left(-\frac{1}{2n\cdot 4^n}\right)=-\frac{1}{2\cdot 4^n}.
$$

äºæ˜¯
$$
\sum_{n=1}^\infty n a_{2n}
=-\frac12\sum_{n=1}^\infty \left(\frac14\right)^n
=-\frac12\cdot \frac{\frac14}{1-\frac14}
=-\frac12\cdot \frac13
=-\frac16.
$$

**ç­”æ¡ˆï¼š$\boxed{-\frac16}$ï¼Œé€‰ (A)ã€‚**
---
Ah â€” **now I see exactly what youâ€™re asking**.
Youâ€™re not asking for arithmetic, youâ€™re asking:

> **Why does the formula use $1-\frac14$ at all? Where does that come from?**

This is an **excellent conceptual question** ğŸ‘
Letâ€™s answer it cleanly.

---

## 1ï¸âƒ£ Where does $1-\frac14$ come from?

It comes from the **geometric series formula**.

For any geometric series
$$
a + ar + ar^2 + ar^3 + \cdots \quad (|r|<1)
$$

the sum is:
$$
\boxed{\frac{a}{1-r}}
$$

ğŸ‘‰ The **$1-r$** is not invented â€” it comes from algebra.

---

## 2ï¸âƒ£ Very short derivation (no tricks)

Let
$$
S = a + ar + ar^2 + ar^3 + \cdots
$$

Multiply both sides by (r):
$$
rS = ar + ar^2 + ar^3 + \cdots
$$

Now subtract:
$$
S - rS = a
$$

Factor:
$$
S(1-r)=a
$$

So:
$$
\boxed{S=\frac{a}{1-r}}
$$

Thatâ€™s it.
**This is why $1-r$ appears.**

---

## 3ï¸âƒ£ Apply this to your specific series

You had:
$$
\sum_{n=1}^\infty \left(\frac14\right)^n
$$

Rewrite it as:
$$
\frac14 + \left(\frac14\right)^2 + \left(\frac14\right)^3 + \cdots
$$

So:

* first term $a=\frac14$
* common ratio $r=\frac14$

Apply the formula:
$$
\sum_{n=1}^\infty \left(\frac14\right)^n
= \frac{a}{1-r}
= \frac{\frac14}{1-\frac14}
$$

ğŸ‘‰ **That is exactly why $1-\frac14$ appears.**

---

## 4ï¸âƒ£ One-sentence intuition (important)

> Each term is only $\tfrac14$ of the previous one,
> so the total sum is controlled by how much is â€œlostâ€ each step â€” that loss is $1-r$.

---

## 5ï¸âƒ£ Final takeaway (memorize this)

Whenever you see:
$$
\sum r^n
\quad\text{or}\quad
\sum ar^n
$$

you should **automatically think**:
$$
\boxed{\text{denominator } = 1-r}
$$

No mystery, no magic â€” just algebra.

If you want, I can also explain:

* why the series **converges only when $|r|<1$**, or
* why the sum becomes **larger** when $r$ is closer to 1

Just tell me ğŸ˜Š

---
Great â€” this is **the right question to ask**.
Letâ€™s clear up **exactly why we expand at (x=0)**, slowly and conceptually.

---

## 1ï¸âƒ£ What does

$$
\sum_{n=0}^\infty a_n x^n
$$
mean?

This is a **power series centered at $x=0$**.

By definition, any series of the form
$$
a_0 + a_1 x + a_2 x^2 + \cdots
$$
is a **Maclaurin series** (Taylor series at $x=0$).

So the sentence

> â€œè®¾å¹‚çº§æ•° $\sum a_n x^n$ çš„å’Œå‡½æ•°ä¸º $\ln(2+x)$â€

means:

> **The Maclaurin series (around $x=0$) of $\ln(2+x)$ has coefficients $a_n$.**

Thatâ€™s **why (x=0) is forced**, not a choice.

---

## 2ï¸âƒ£ Why do we rewrite $\ln(2+x)$?

We know a **standard Maclaurin expansion**:

$$
\boxed{\ln(1+t)=\sum_{m=1}^\infty (-1)^{m+1}\frac{t^m}{m}}
\quad (|t|<1)
$$

So we try to make $\ln(2+x)$ look like $\ln(1+t)$.

---

## 3ï¸âƒ£ Factor out the 2 (this is the key trick)

$$
\ln(2+x)=\ln(2(1+\frac x2))
$$

Using log rules:

$$
\ln(2+x)=\ln2+\ln\left(1+\frac x2\right)
$$

Now it matches the known formula with
$$
t=\frac x2
$$

---

## 4ï¸âƒ£ Now expand at (x=0)

$$
\ln\left(1+\frac x2\right)
=\sum_{m=1}^\infty (-1)^{m+1}\frac1m\left(\frac x2\right)^m
\quad(|x|<2)
$$

So the full expansion is:

$$
\ln(2+x)=\ln2+\sum_{m=1}^\infty (-1)^{m+1}\frac{x^m}{m2^m}
$$

---

## 5ï¸âƒ£ How do we â€œread offâ€ the coefficients (a_n)?

Compare with:

$$
\sum_{n=0}^\infty a_n x^n
$$

We immediately see:

* $a_0=\ln2$
* For $n\ge1$:
  $$
  \boxed{a_n = (-1)^{n+1}\frac{1}{n2^n}}
  $$

Thatâ€™s how we â€œknowâ€ the coefficients.

---

## 6ï¸âƒ£ One-sentence takeaway (very important)

> **Whenever you see $\sum a_n x^n$, the expansion is automatically about $x=0$.**

If the problem wanted expansion at another point, it would say something like
$\sum a_n (x-1)^n$.

---

If you want, I can also show:

* how this relates to derivatives at $x=0$, or
* how to do the same problem *without* explicitly finding all $a_n$

Just tell me ğŸ‘

---

Great question â€” this is a **terminology issue**, not a math skill issue ğŸ‘
Once this is clear, many problems will suddenly make sense.

---

## What does **â€œå’Œå‡½æ•°â€** mean?

In Chinese math language:

> **å¹‚çº§æ•°çš„å’Œå‡½æ•°** = **the function represented by the power series**

Formally:

If
$$
\sum_{n=0}^\infty a_n x^n
$$
converges for some $x$, and its sum equals a function $f(x)$, then

$$
\boxed{f(x)\ \text{is called the å’Œå‡½æ•° of the series}}
$$

---

## In plain English

* The **power series** is:
 $$
  a_0 + a_1 x + a_2 x^2 + \cdots
 $$

* The **å’Œå‡½æ•°** is:
 $$
  f(x)=a_0 + a_1 x + a_2 x^2 + \cdots
 $$

So â€œå’Œå‡½æ•°â€ just means:

> **the function you get after adding up all the infinitely many terms**

---

## Example 1 (very familiar)

$$
\sum_{n=0}^\infty x^n
$$

This series converges for (|x|<1), and:

$$
\sum_{n=0}^\infty x^n=\frac1{1-x}
$$

So:

* å¹‚çº§æ•°ï¼š$\sum x^n$
* å’Œå‡½æ•°ï¼š$\displaystyle \frac1{1-x}$

---

## Example 2 (your problem)

The problem says:

> è®¾å¹‚çº§æ•° $\sum a_n x^n$ çš„å’Œå‡½æ•°ä¸º $\ln(2+x)$

That means:

$$
\boxed{\sum_{n=0}^\infty a_n x^n = \ln(2+x)\quad(\text{åœ¨æ”¶æ•›åŒºé—´å†…})}
$$

So **$\ln(2+x)$** is the function obtained after summing the series.

---

## Why this matters

This tells you:

* the series is a **Maclaurin series**
* its coefficients $a_n$ are exactly the Maclaurin coefficients of $\ln(2+x)$

Thatâ€™s why we are allowed to expand $\ln(2+x)$ and compare terms.

---

## One-line memory rule ğŸ§ 

> **â€œå’Œå‡½æ•°â€ = â€œthe function whose value equals the sum of the seriesâ€**

---

If you want, I can also explain:

* the difference between **å’Œå‡½æ•°** and **é€šé¡¹**, or
* how to check the **æ”¶æ•›åŒºé—´**

Just tell me ğŸ˜Š

---
Yes â€” **exactly right** ğŸ‘
In *this problem*, **$a = \tfrac14$**. Let me show you **why**, step by step, tied directly to the expression you saw.

---

## 1ï¸âƒ£ The geometric series formula

For a geometric series
$$
a + ar + ar^2 + \cdots
$$
the sum is
$$
\frac{a}{1-r}
$$

Here:

* $a$ = **first term**
* $r$ = **common ratio**

---

## 2ï¸âƒ£ Look at the series you actually had

From the solution:
$$
\sum_{n=1}^\infty \left(\frac14\right)^n
$$

Write out the first few terms:
$$
\left(\frac14\right)^1

+ \left(\frac14\right)^2
+ \left(\frac14\right)^3
+ \cdots
$$

That is:
$$
\frac14 + \frac1{16} + \frac1{64} + \cdots
$$

---

## 3ï¸âƒ£ Identify (a) and (r)

* The **first term** is:
  $$
  a = \frac14
  $$

* Each term is multiplied by $\frac14$ to get the next one, so:
  $$
  r = \frac14
  $$

Thatâ€™s why **both** $a$ and $r$ are $\frac14$ here.

---

## 4ï¸âƒ£ Apply the formula

$$
\sum_{n=1}^\infty \left(\frac14\right)^n
= \frac{a}{1-r}
= \frac{\frac14}{1-\frac14}
$$

This is **not a coincidence** â€” it comes directly from identifying the first term.

---

## 5ï¸âƒ£ Why this mattered in the full problem

You had:
$$
\sum_{n=1}^\infty n a_{2n}
= -\frac12 \sum_{n=1}^\infty \left(\frac14\right)^n
$$

So:
$$
-\frac12 \cdot \frac{\frac14}{1-\frac14}
= -\frac12 \cdot \frac13
= -\frac16
$$

---

## Final takeaway (very important)

> In $\dfrac{a}{1-r}$,
> **$a$ is always the first term of the series**, not a random number.

So yes â€” **in this problem, $a = \tfrac14$** âœ”ï¸

If you want, I can next explain **why the sum starts at $n=1$ instead of $n=0$**, which is another common confusion.

---

This is a **very common and very important confusion** â€” youâ€™re thinking correctly, just mixing **two different series**. Letâ€™s separate them cleanly.

---

## 1ï¸âƒ£ What *is* the series we are summing?

The series in the problem is:

$$
\sum_{n=1}^\infty \left(\frac14\right)^n
$$

**Look carefully:**
ğŸ‘‰ it starts at **$n=1$**, **not $n=0$**.

---

## 2ï¸âƒ£ Write out the actual terms

Substitute values of $n$:

* when $n=1$: $\left(\frac14\right)^1=\frac14$
* when $n=2$: $\left(\frac14\right)^2=\frac1{16}$
* when $n=3$: $\left(\frac14\right)^3=\frac1{64}$

So the series is:
$$
\frac14+\frac1{16}+\frac1{64}+\cdots
$$

âœ… **The first term is $\frac14$**.

---

## 3ï¸âƒ£ Where does $\left(\frac14\right)^0=1$ belong?

That term appears in a **different series**:

$$
\sum_{n=0}^\infty \left(\frac14\right)^n
= 1+\frac14+\frac1{16}+\cdots
$$

Here:

* first term $=1$
* this is **not** the series we are summing

So your statement is correct **for a different series**, but **not for this one**.

---

## 4ï¸âƒ£ Why does the geometric-series formula still work?

The standard formula
$$
\frac{a}{1-r}
$$
assumes the series is:
$$
a+ar+ar^2+\cdots
$$

In our case:
$$
\frac14+\frac1{16}+\frac1{64}+\cdots
$$

So:

* $a=\frac14$
* $r=\frac14$

Thatâ€™s why:
$$
\sum_{n=1}^\infty \left(\frac14\right)^n
=\frac{\frac14}{1-\frac14}
$$

---

## 5ï¸âƒ£ Key rule to remember (this clears everything)

> **The â€œfirst termâ€ is the term with the smallest index actually used.**

* starts at (n=0) â†’ first term is (r^0=1)
* starts at (n=1) â†’ first term is (r^1=r)

---

## âœ… Final conclusion

* Your thought **â€œ$(1/4)^0=1$â€ is mathematically correct**
* But **that term is not in this series**
* Therefore, for **this problem**, the first term is:
  $$
  \boxed{\frac14}
  $$

Youâ€™re doing great â€” this confusion happens to almost everyone once.

---

Great â€” this is a **definition-level question**, and once it clicks, everything else becomes automatic.

You are asking **why**
$$
(Qv)\cdot(Qv) = (Qv)^T(Qv).
$$

Letâ€™s explain this **from the ground up**, with no shortcuts.

---

## 1ï¸âƒ£ What is the dot product, really?

Take two vectors in $\mathbb{R}^n$:
$$
a=\begin{pmatrix}a_1\\a_2\\\vdots\\a_n\end{pmatrix},
\quad
b=\begin{pmatrix}b_1\\b_2\\\vdots\\b_n\end{pmatrix}.
$$

By definition, their **dot product** is:
$$
a\cdot b = a_1b_1 + a_2b_2 + \cdots + a_nb_n.
$$

---

## 2ï¸âƒ£ How does transpose + matrix multiplication encode this?

Write $a$ as a **column vector**.
Then its transpose $a^T$ is a **row vector**:
$$
a^T = (a_1\ a_2\ \cdots\ a_n).
$$

Now multiply:
$$
a^Tb
=

(a_1\ a_2\ \cdots\ a_n)
\begin{pmatrix}b_1\\b_2\\\vdots\\b_n\end{pmatrix}
=

a_1b_1 + a_2b_2 + \cdots + a_nb_n.
$$

So we get:
$$
\boxed{a\cdot b = a^Tb}
$$

This is **not a trick** â€” it is exactly the same operation written in matrix form.

---

## 3ï¸âƒ£ Apply this to your case

Let
[
w = Qv.
]

Then (w) is just a vector, so by the rule above:
[
w\cdot w = w^Tw.
]

Substitute back:
[
(Qv)\cdot(Qv) = (Qv)^T(Qv).
]

Thatâ€™s it.

---

## 4ï¸âƒ£ Why mathematicians do this (important intuition)

Writing dot products as (v^Tv) lets us:

* combine dot products with matrices
* use transpose rules
* prove properties like length preservation cleanly

For example:
[
(Qv)^T(Qv) = v^TQ^TQv
]

This step would be **impossible** without the transpose form.

---

## 5ï¸âƒ£ One-sentence takeaway ğŸ§ 

> **Dot product = transpose Ã— column product**

or
[
\boxed{a\cdot b = a^Tb}
]

Everything else follows from this identity.

If you want, next I can explain **why transpose behaves the way it does** (e.g. why ((AB)^T=B^TA^T)), which is the next logical step.













